backend/RenumberproofC.v
@@ -6,7 +6,7 @@ Require Import sflib.
 (** newly added **)
 Require Export Renumberproof.
 Require Import Simulation.
-Require Import Skeleton Mod ModSem SimMod SimModSem SimSymbId SimMemId SimMem AsmregsC MatchSimModSem.
+Require Import Skeleton Mod ModSem SimMod SimModSem SimSymb SimSymbId SimMem SimMemId AsmregsC MatchSimModSem.
 
 Set Implicit Arguments.
 
@@ -24,7 +24,9 @@ Section RNMBREXTRA.
   (* Let tge := Genv.globalenv tprog. *)
   Variable ge tge: genv.
 
-  Lemma step_simulation (SIMGE: False):
+  Lemma step_simulation
+        (SIMGE: Genv.match_genvs (match_globdef (fun _ f tf => tf = transf_fundef f) eq prog) ge tge)
+    :
   forall S1 t S2 (NOTEXT: ~ RTLC.is_external ge S1), Step (semantics_with_ge prog ge) S1 t S2 ->
   forall S1', match_states S1 S1' ->
   exists S2', DStep (semantics_with_ge tprog tge) S1' t S2' /\ match_states S2 S2'.
@@ -35,6 +37,185 @@ Section RNMBREXTRA.
 End RNMBREXTRA.
 
 
+
+Section MATCHEXTRA.
+
+  Context {C F1 V1 F2 V2: Type} {LC: Linker C} {LF: Linker F1} {LV: Linker V1}.
+  Variable match_fundef: C -> AST.fundef F1 -> AST.fundef F2 -> Prop.
+  Variable match_varinfo: V1 -> V2 -> Prop.
+  Hypothesis MATCH_FUNDEF_EXTERNAL: forall
+      ctx f_src f_tgt
+      (MATCH: match_fundef ctx f_src f_tgt)
+    ,
+      is_external_fd f_src = is_external_fd f_tgt
+  .
+
+  Variables (ctx: C) (p_src: AST.program (AST.fundef F1) V1) (p_tgt: AST.program (AST.fundef F2) V2).
+
+  Lemma match_program_gen_defs
+        (MATCH: match_program_gen match_fundef match_varinfo ctx p_src p_tgt)
+    :
+      <<EQ: p_src.(defs) = p_tgt.(defs)>>
+  .
+  Proof.
+    apply Axioms.functional_extensionality. ii; ss. u.
+    (* hexploit (match_program_defmap _ _ ctx p_src p_tgt MATCH x). intro REL. *)
+    inv MATCH. des.
+    assert((prog_defs_names p_src) = (prog_defs_names p_tgt)).
+    { unfold prog_defs_names.
+      clear - H.
+      ginduction H; ii; ss.
+      inv H; ss. f_equal; ss.
+    }
+    rewrite H2; ss.
+  Qed.
+
+  Lemma match_program_gen_preserves_sim_skenv
+        skenv_link_src skenv_link_tgt
+        (SIMSKENV: SimSymbId.sim_skenv skenv_link_src skenv_link_tgt)
+        (MATCH: match_program_gen match_fundef match_varinfo ctx p_src p_tgt)
+        proj_src proj_tgt
+        (PROJSRC: SkEnv.project_spec skenv_link_src p_src.(defs) proj_src)
+        (PROJTGT: SkEnv.project_spec skenv_link_tgt p_tgt.(defs) proj_tgt)
+    :
+      <<SIMSKENV: SimSymbId.sim_skenv proj_src proj_tgt>>
+  .
+  Proof.
+    clarify. inv SIMSKENV. inv PROJSRC. inv PROJTGT.
+    econs; eauto.
+    - eq_closure_tac.
+    - ii; ss.
+      destruct (defs p_src x0) eqn:T.
+      + erewrite SYMBKEEP; eauto.
+        erewrite SYMBKEEP0; eauto.
+        erewrite <- match_program_gen_defs; eauto.
+      + erewrite SYMBDROP; eauto.
+        erewrite SYMBDROP0; eauto.
+        erewrite <- match_program_gen_defs; eauto.
+        congruence.
+        congruence.
+    - intro blk.
+      destruct (Genv.invert_symbol skenv_link_src blk) eqn:T0; cycle 1.
+      + rewrite DEFORPHAN; ss.
+        destruct (Genv.invert_symbol skenv_link_tgt blk) eqn:T1; cycle 1.
+        * rewrite DEFORPHAN0; ss.
+        * repeat all_once_fast ltac:(fun H => try apply Genv.invert_find_symbol in H; des).
+          rewrite <- SYMB in *.
+          repeat all_once_fast ltac:(fun H => try apply Genv.find_invert_symbol in H; des).
+          clarify.
+      + destruct (Genv.invert_symbol skenv_link_tgt blk) eqn:T1; cycle 1.
+        * repeat all_once_fast ltac:(fun H => try apply Genv.invert_find_symbol in H; des).
+          rewrite SYMB in *.
+          repeat all_once_fast ltac:(fun H => try apply Genv.find_invert_symbol in H; des).
+          clarify.
+        * repeat all_once_fast ltac:(fun H => try apply Genv.invert_find_symbol in H; des).
+          assert(i = i0).
+          { eapply Genv.genv_vars_inj; eauto. unfold Genv.find_symbol in *. rewrite SYMB. ss. }
+          clarify.
+          repeat all_once_fast ltac:(fun H => try apply Genv.find_invert_symbol in H; des).
+          destruct (classic (defs p_src i0)).
+          { erewrite DEFKEEP; eauto. erewrite DEFKEEP0; eauto. erewrite <- match_program_gen_defs; eauto. }
+          { erewrite DEFDROP; eauto. erewrite DEFDROP0; eauto. erewrite <- match_program_gen_defs; eauto. }
+  Admitted. (* COQ BUG!!!!!!!!!!!!!!!! HOW TO FIX THIS?????????? *)
+
+  Lemma o_bind_assertion
+        X Y
+        (x: option X) (y: option Y)
+    :
+      (do _ <- x ; y) = assertion(x) ; y
+  .
+  Proof. u. des_ifs. Qed.
+
+  Lemma match_globdef_external
+        x y
+        (MATCH: match_globdef match_fundef match_varinfo ctx x y)
+    :
+      <<EQ: is_external x = is_external y>>
+  .
+  Proof. inv MATCH; ss. eapply MATCH_FUNDEF_EXTERNAL; eauto. Qed.
+
+  Lemma match_program_gen_revive_match_genvs
+        skenv_link_src skenv_link_tgt
+        (SIMSKENV: SimSymbId.sim_skenv skenv_link_src skenv_link_tgt)
+        (MATCH: match_program_gen match_fundef match_varinfo ctx p_src p_tgt)
+        proj_src proj_tgt
+        (PROJSRC: SkEnv.project_spec skenv_link_src p_src.(defs) proj_src)
+        (PROJTGT: SkEnv.project_spec skenv_link_tgt p_tgt.(defs) proj_tgt)
+        ge_src ge_tgt
+        (REVIVESRC: ge_src = SkEnv.revive proj_src p_src)
+        (REVIVETGT: ge_tgt = SkEnv.revive proj_tgt p_tgt)
+    :
+      <<SIMGE: Genv.match_genvs (match_globdef match_fundef match_varinfo ctx) ge_src ge_tgt>>
+  .
+  Proof.
+    exploit match_program_gen_preserves_sim_skenv; eauto. intro SIMSKENVPROJ; des. inv SIMSKENVPROJ.
+    econs; eauto.
+    intro blk; ss.
+    inv PROJSRC. inv PROJTGT. rewrite ! MapsC.PTree_filter_map_spec in *.
+    {
+      rewrite ! o_bind_assertion.
+      destruct (Genv.invert_symbol proj_src blk) eqn:T0; cbn; cycle 1.
+      - destruct (Genv.invert_symbol proj_tgt blk) eqn:T1; cbn; cycle 1.
+        + u. des_ifs; econs; eauto.
+        + repeat all_once_fast ltac:(fun H => try apply Genv.invert_find_symbol in H; des).
+          erewrite <- SYMB in *.
+          repeat all_once_fast ltac:(fun H => try apply Genv.find_invert_symbol in H; des).
+          clarify.
+      - repeat all_once_fast ltac:(fun H => try apply Genv.invert_find_symbol in H; des).
+        dup T0.
+        rewrite SYMB in T1.
+        repeat all_once_fast ltac:(fun H => try apply Genv.find_invert_symbol in H; des).
+        rewrite T1. cbn.
+        rename i into id.
+        specialize (DEFS blk).
+        unfold Genv.find_def in *.
+        des_ifs; clarify; cycle 1.
+        { econs; eauto. }
+        apply match_program_defmap with (id0 := id) in MATCH.
+        inv MATCH; cbn.
+        { econs; eauto. }
+        erewrite match_globdef_external; eauto.
+        des_ifs; econs; eauto.
+    }
+  Admitted. (* COQ BUG!!!!!!!!!!!!!!!! HOW TO FIX THIS?????????? *)
+
+  Lemma match_program_gen_revive_match_genvs_deprecated
+        skenv_link_src skenv_link_tgt
+        (SIMSKENV: SimSymbId.sim_skenv skenv_link_src skenv_link_tgt)
+        (MATCH: match_program_gen match_fundef match_varinfo ctx p_src p_tgt)
+        ge_src ge_tgt
+        (REVIVESRC: ge_src = SkEnv.revive (SkEnv.project skenv_link_src (defs p_src)) p_src)
+        (REVIVETGT: ge_tgt = SkEnv.revive (SkEnv.project skenv_link_tgt (defs p_tgt)) p_tgt)
+    :
+      <<SIMGE: Genv.match_genvs (match_globdef match_fundef match_varinfo ctx) ge_src ge_tgt>>
+  .
+  Proof.
+    clarify. dup MATCH. inv MATCH. des; ss. inv SIMSKENV. ss.
+    hexploit (@SkEnv.project_impl_spec skenv_link_src p_src.(defs)). intro SPECSRC.
+    hexploit (@SkEnv.project_impl_spec skenv_link_tgt p_tgt.(defs)). intro SPECTGT.
+    abstr ((SkEnv.project skenv_link_src (defs p_src))) proj_src.
+    abstr ((SkEnv.project skenv_link_tgt (defs p_tgt))) proj_tgt.
+    (* set ((SkEnv.project skenv_link_src (defs p_src))) as proj_src in *. *)
+    (* set ((SkEnv.project skenv_link_tgt (defs p_tgt))) as proj_tgt in *. *)
+    inv SPECSRC. inv SPECTGT.
+    {
+      econs; eauto.
+      - unfold SkEnv.revive. unfold Genv_map_defs. simpl. eq_closure_tac.
+      - i. u. ss.
+        unfold Genv.find_symbol in *.
+        destruct (defs p_src id) eqn:T.
+        + erewrite SYMBKEEP; eauto.
+          erewrite SYMBKEEP0; eauto.
+          erewrite <- match_program_gen_defs; eauto.
+        + erewrite SYMBDROP; eauto.
+          erewrite SYMBDROP0; eauto.
+          erewrite <- match_program_gen_defs; eauto.
+          congruence.
+          congruence.
+      - ii.
+  Abort.
+
+End MATCHEXTRA.
 
 
 
@@ -114,7 +295,13 @@ Proof.
     inv MATCH.
     apply Axioms.functional_extensionality in SIMRSINIT. clarify.
     ii. hexploit (@step_simulation prog tprog ge tge); eauto.
-    { admit "WE SHOULD ADDRESS THIS". }
+    { unfold match_prog, match_program in *.
+      eapply match_program_gen_revive_match_genvs; [| |unshelve eapply TRANSL; eauto|..].
+      { ii; ss. clarify. u. des_ifs. }
+      admit "".
+      admit "".
+      apply TRANSL.
+      admit "WE SHOULD ADDRESS THIS". }
     { apply not_external. }
     i; des.
     esplits; eauto.
